Skip programs

CircuitComp/BranchingProgram/Basic.lean
@@ -24,12 +24,12 @@ Two assumptions this form does not make:
   matters quite a bit.
 -/
 structure LayeredBranchingProgram (α : Type u) (β : Type v) (γ : Type w) where
-  /- The number of layers in the program. We use the convention that `depth = 0` means
+  /-- The number of layers in the program. We use the convention that `depth = 0` means
   that there is only the input layer; this avoids some awkward issues with `NeZero depth`
   instances or tracking when an index is properly in bounds. -/
   depth : ℕ
-  /- The set of nodes in each layer. -/
-  nodes (n : Fin depth.succ) : Type v
+  /-- The set of nodes in each layer. -/
+  nodes (n : Fin (depth + 1)) : Type v
   /- The variable that each node depends on. -/
   nodeVar {n : Fin depth} : nodes n.castSucc → α
   /- The outgoing edges from each node. -/
@@ -37,6 +37,34 @@ structure LayeredBranchingProgram (α : Type u) (β : Type v) (γ : Type w) wher
   /- The proposition that the starting node is unique.-/
   startUnique : Unique (nodes 0)
   /- The end nodes each return a value in `γ`. -/
+  retVals : nodes (Fin.last depth) → γ
+
+/--
+An unlayered and unstructured branching program, represented as a DAG.
+Compared with `LayeredBranchingProgram`, this allows for infinite branching programs
+and input-dependent, unbounded depths.
+-/
+structure BranchingProgram (α : Type u) (β : Type v) (γ : Type w) where
+  nodes : Type v
+  start : nodes
+  /-- Every node either returns a value in `γ`, or reads a variable `α` and branches to the next node. -/
+  info : nodes → γ ⊕ (α × (β → nodes))
+  /-- The relation `child` is well-founded, ensuring no infinite paths. -/
+  wellFounded : WellFounded (fun v u ↦ ∃ var next val, info u = .inr (var, next) ∧ next val = v)
+
+/-
+A `SkipBranchingProgram` is similar to `LayeredBranchingProgram`, but allows for skipping layers:
+a node at layer `n` can skip to any layer `m` with `n < m`. This is largely equivalent
+computationally, but allows for a reduction in width in some cases.
+-/
+structure SkipBranchingProgram (α : Type u) (β : Type v) (γ : Type w) where
+  depth : ℕ
+  nodes (n : Fin (depth + 1)) : Type v
+  nodeVar {n : Fin depth} : nodes n.castSucc → α
+  edges {n : Fin depth} : nodes n.castSucc → β → Σ (m : Fin (depth + 1)), nodes m
+  edges_layer_gt {n : Fin depth} (u : nodes n.castSucc) (b : β) :
+    n.castSucc < (edges u b).1
+  startUnique : Unique (nodes 0)
   retVals : nodes (Fin.last depth) → γ
 
 namespace LayeredBranchingProgram
@@ -122,13 +150,13 @@ def computes (F : (α → β) → γ) : Prop :=
 /--
 Evaluation for `LayeredBranchingProgram` starting from a specific layer and node.
 -/
-def evalFrom (P : LayeredBranchingProgram α β γ) (x : α → β) (i : Fin P.depth.succ) (u : P.nodes i) : γ :=
+def evalAt (P : LayeredBranchingProgram α β γ) (x : α → β) (i : Fin P.depth.succ) (u : P.nodes i) : γ :=
   if h : i = Fin.last P.depth then
     P.retVals (h ▸ u)
   else
     let i' : Fin P.depth := i.castPred h
     let u' : P.nodes i'.castSucc := (Fin.castSucc_castPred i h).symm ▸ u
-    evalFrom P x i'.succ (P.edges u' (x (P.nodeVar u')))
+    evalAt P x i'.succ (P.edges u' (x (P.nodeVar u')))
   termination_by P.depth - i
   decreasing_by
     have h_i_lt_depth : i.val < P.depth :=
@@ -137,15 +165,15 @@ def evalFrom (P : LayeredBranchingProgram α β γ) (x : α → β) (i : Fin P.d
     omega
 
 /--
-`evalFrom` starting at the node reached by `evalLayer` yields the same result as `eval`.
+`evalAt` starting at the node reached by `evalLayer` yields the same result as `eval`.
 -/
 @[simp]
-theorem evalFrom_evalLayer_eq_eval (x : α → β) (i : Fin P.depth.succ) :
-    P.evalFrom x i (P.evalLayer i x) = P.eval x := by
+theorem evalAt_evalLayer_eq_eval (x : α → β) (i : Fin P.depth.succ) :
+    P.evalAt x i (P.evalLayer i x) = P.eval x := by
   induction i using Fin.reverseInduction
-  · simp [eval, evalFrom]
+  · simp [eval, evalAt]
   · rename_i i ih
-    unfold evalFrom
+    unfold evalAt
     simpa using ih
 
 end LayeredBranchingProgram
@@ -176,7 +204,7 @@ def BPFamily.hasWidth (w : GrowthRate) : Prop :=
 protected class BPFamily.Finite : Prop where
   finite : ∀ n, (BPF n).Finite
 
-instance [inst : BPFamily.Finite BPF] {n} : (BPF n).Finite :=
+instance [inst : BPF.Finite] {n} : (BPF n).Finite :=
   inst.finite n
 
 /-- Predicate expressing that the size grows as O(f n). -/
@@ -198,43 +226,72 @@ def BPClass (width : GrowthRate) (depth : GrowthRate) (obliv : Bool) : Set (Func
     ∧ (obliv → BPF.IsOblivious)
 
 variable [BPF.Finite] {w : ℕ}
-/--
-The size of a branching program in a family with bounded width is bounded by width * depth + 1.
--/
+
+/-- The size of a branching program in a family with bounded width is bounded by width * depth + 1. -/
 theorem BPFamily.size_le_bound (hw : BPF.hasWidth (·≤w)) :
     ∀ n, (BPF n).size ≤ w * (BPF n).depth + 1 := by
   intro n
   grw [(BPF n).size_le_width_mul_depth, show (BPF n).width ≤ w from hw n]
 
-/--
-If a branching program family has constant width and polynomial depth, it has polynomial size.
--/
+/-- If a branching program family has constant width and polynomial depth, it has polynomial size. -/
 theorem BPFamily.hasSize_poly_of_width_depth (hw : BPF.hasWidth (·≤w)) (hd : BPF.hasDepth .poly) :
     BPF.hasSize GrowthRate.poly :=
   GrowthRate.mono (GrowthRate.affine_comp hd) (BPF.size_le_bound hw)
 
 end BPFamily
 
-/--
-An unlayered and unstructured branching program, represented as a DAG.
-Compared with `LayeredBranchingProgram`, this allows for infinite branching programs
-and input-dependent, unbounded depths.
--/
-structure BranchingProgram (α : Type u) (β : Type v) (γ : Type w) where
-  nodes : Type v
-  start : nodes
-  info : nodes → Sum γ (α × (β → nodes))
-  /-- The relation `child` is well-founded, ensuring no infinite paths. -/
-  wellFounded : WellFounded (fun v u ↦ ∃ var next val, info u = .inr (var, next) ∧ next val = v)
+namespace SkipBranchingProgram
+
+variable {α : Type u} {β : Type v} {γ : Type w} (P : SkipBranchingProgram α β γ)
+
+attribute [instance] startUnique
+
+def start : P.nodes 0 :=
+  P.startUnique.default
+
+/-- We call a skip branching program finite if the nodes at each layer is finite. -/
+protected class Finite : Prop where
+  finite : ∀ i, Finite (P.nodes i)
+
+instance [inst : P.Finite] {i} : Finite (P.nodes i) :=
+  inst.finite i
+
+/-- Evaluate a `SkipBranchingProgram` starting from a specific node. -/
+def evalAt (P : SkipBranchingProgram α β γ) (x : α → β) {i : Fin P.depth.succ} (u : P.nodes i) : γ :=
+  if h : i = Fin.last P.depth then
+    P.retVals (h ▸ u)
+  else
+    let i' : Fin P.depth := i.castPred h
+    let u' : P.nodes i'.castSucc := (Fin.castSucc_castPred i h).symm ▸ u
+    let next := P.edges u' (x (P.nodeVar u'))
+    P.evalAt x next.2
+  termination_by P.depth - i
+  decreasing_by
+    simp_wf
+    have h_lt : i.val < P.depth := by
+      have h_le : i.val ≤ P.depth := by omega
+      have h_ne : i.val ≠ P.depth := by
+        contrapose! h
+        apply Fin.eq_of_val_eq h.1
+      omega
+    let i' : Fin P.depth := i.castPred h
+    let u' : P.nodes i'.castSucc := (Fin.castSucc_castPred i h).symm ▸ u
+    have h_gt := P.edges_layer_gt u' (x (P.nodeVar u'))
+    simp only [i', u'] at h_gt
+    apply Nat.sub_lt_sub_left h_lt h_gt
+
+/-- Evaluate a `SkipBranchingProgram` on inputs `x`. -/
+def eval (x : α → β) : γ :=
+  P.evalAt x P.start
+
+end SkipBranchingProgram
 
 namespace BranchingProgram
 
 variable {α : Type u} {β : Type v} {γ : Type w}
 variable (P : BranchingProgram α β γ)
 
-/--
-Evaluation for `BranchingProgram` starting from a specific node.
--/
+/-- Evaluation for `BranchingProgram` starting from a specific node. -/
 def evalAt (x : α → β) (u : P.nodes) : γ :=
   P.wellFounded.fix (fun u ih ↦
     match h : P.info u with
@@ -242,12 +299,126 @@ def evalAt (x : α → β) (u : P.nodes) : γ :=
     | .inr (var, next) => ih (next (x var)) ⟨var, next, x var, h, rfl⟩
   ) u
 
-/--
-Evaluation for `BranchingProgram`.
--/
+/-- Evaluation for `BranchingProgram`. -/
 def eval (x : α → β) : γ :=
   P.evalAt x P.start
 
+section height
+
+open Classical
+variable [Fintype P.nodes]
+
+/-- The height of a node in a branching program is the length of the longest path to a leaf. -/
+noncomputable def height (u : P.nodes) : ℕ :=
+  letI := Fintype.ofFinite P.nodes
+  P.wellFounded.fix (fun u ih ↦
+    match h : P.info u with
+    | .inl _ => 0
+    | .inr (var, next) =>
+      let children := Finset.univ.filter (fun v ↦ ∃ b, next b = v)
+      1 + children.attach.sup (fun (v : {x // x ∈ children}) ↦
+          ih v.1 (by
+            have hv := v.2
+            rw [Finset.mem_filter] at hv
+            rcases hv with ⟨_, ⟨b, hb⟩⟩
+            exact ⟨var, next, b, h, hb⟩
+          )
+      )
+  ) u
+
+/-- The depth of a branching program is the height of the start node. -/
+noncomputable def depth : ℕ :=
+  P.height P.start
+
+theorem height_eq_zero_of_leaf (u : P.nodes) (res : γ)
+    (h : P.info u = .inl res) : P.height u = 0 := by
+  grind [WellFounded.fix_eq, height]
+
+theorem height_eq_succ_sup (u : P.nodes) (var : α) (next : β → P.nodes) (h : P.info u = .inr (var, next)) :
+    P.height u = 1 + (Finset.univ.filter (fun v ↦ ∃ b, next b = v)).sup (fun v ↦ P.height v) := by
+  rw [height, WellFounded.fix_eq]
+  simp only [Finset.sup_attach]
+  rw [h]
+  convert rfl
+
+theorem height_pos (u : P.nodes) (var : α) (next : β → P.nodes) (h : P.info u = .inr (var, next)) :
+    0 < P.height u := by
+  have h_height_def : P.height u = 1 + (Finset.univ.filter (fun v ↦ ∃ b, next b = v)).sup (fun v ↦ P.height v) := by
+    exact height_eq_succ_sup P u var next h;
+  exact h_height_def.symm ▸ add_pos_of_pos_of_nonneg zero_lt_one ( Nat.zero_le _ )
+
+theorem is_internal_of_height_pos (u : P.nodes)
+    (h : 0 < P.height u) : ∃ var next, P.info u = .inr (var, next) := by
+  rcases h : P.info u with (_  | ⟨_, _⟩)
+  · have := height_eq_zero_of_leaf P _ _ h
+    linarith
+  · simp
+
+theorem is_leaf_of_height_zero (u : P.nodes)
+    (h : P.height u = 0) : ∃ res, P.info u = .inl res := by
+  by_contra h_contra;
+  have h_height_pos : 0 < P.height u := by
+    -- Since u is not a leaf, its info is .inr (var, next).
+    obtain ⟨var, next, h_info⟩ : ∃ var next, P.info u = .inr (var, next) := by
+      cases h : P.info u <;> tauto;
+    convert P.height_pos u var next h_info
+  grind
+
+theorem height_child_lt (u : P.nodes) (var : α) (next : β → P.nodes) (h : P.info u = .inr (var, next)) (b : β) :
+    P.height (next b) < P.height u := by
+  rw [height_eq_succ_sup P u var next h, add_comm, Nat.lt_add_one_iff]
+  exact Finset.le_sup (by simp)
+
+theorem leaf_of_layer_eq_depth (u : P.nodes) (h : P.height u = P.depth - P.depth) :
+    ∃ res, P.info u = .inl res :=
+  P.is_leaf_of_height_zero u (by omega)
+
+end height
+
+section rel
+open Relation
+
+def adj (u v : P.nodes) : Prop :=
+  ∃ var next, P.info u = .inr (var, next) ∧ ∃ b, next b = v
+
+def Reachable (u : P.nodes) : Prop :=
+  ReflTransGen P.adj P.start u
+
+variable [Fintype P.nodes]
+
+theorem height_lt_of_adj {u v : P.nodes}
+    (h : P.adj u v) : P.height v < P.height u := by
+  rcases h with ⟨var, next, hx, b, rfl⟩;
+  convert BranchingProgram.height_child_lt P u var next hx b
+
+theorem height_le_of_reachable {u : P.nodes}
+    (h : P.Reachable u) : P.height u ≤ P.height P.start := by
+  cases h ; aesop;
+  rename_i b hb₁ hb₂;
+  have h_adj_anti : ∀ c d : P.nodes, P.adj c d → P.height d < P.height c := by
+    intro c d hcd
+    obtain ⟨var, next, hinfo, ⟨b, hb⟩⟩ := hcd
+    have h_height_lt : P.height (next b) < P.height c := by
+      convert P.height_child_lt c var next hinfo b using 1
+    aesop;
+  have h_adj_anti : ∀ c d : P.nodes, ReflTransGen P.adj c d → P.height d ≤ P.height c := by
+    intro c d hcd; induction hcd <;> [ rfl; linarith [ h_adj_anti _ _ ‹_› ] ] ;
+  exact le_trans ( h_adj_anti _ _ ( ReflTransGen.single hb₂ ) ) ( h_adj_anti _ _ hb₁ )
+
+theorem eq_start_of_reachable_and_height_eq {u : P.nodes}
+    (h : P.Reachable u) (heq : P.height u = P.height P.start) : u = P.start := by
+  have h_height_u : u ≠ P.start → P.height u < P.height P.start := by
+    intro hu
+    have h_height_u : ∀ v : P.nodes, P.Reachable v → v ≠ P.start → P.height v < P.height P.start := by
+      intro w hw hw_ne_start
+      induction hw
+      · contradiction
+      · have _ := height_lt_of_adj P ‹_›
+        grind
+    exact h_height_u u h hu;
+  exact Classical.not_not.1 fun h' => heq.not_lt <| h_height_u h'
+
+end rel
 end BranchingProgram
 
 namespace LayeredBranchingProgram
@@ -280,16 +451,16 @@ def toBranchingProgram : BranchingProgram α β γ where
       exact ih (L.edges u x)
 
 /--
-`evalAt` on the converted DAG equals `evalFrom` on the layered program.
+`evalAt` on the converted DAG equals `evalAt` on the layered program.
 -/
-theorem toBranchingProgram_evalAt_eq_evalFrom (x : α → β) (i : Fin L.depth.succ) (u : L.nodes i) :
-    L.toBranchingProgram.evalAt x ⟨i, u⟩ = L.evalFrom x i u := by
+theorem toBranchingProgram_evalAt_eq_evalAt (x : α → β) (i : Fin L.depth.succ) (u : L.nodes i) :
+    L.toBranchingProgram.evalAt x ⟨i, u⟩ = L.evalAt x i u := by
   induction' i using Fin.reverseInduction with i ih;
-  · rw [ evalFrom ];
+  · rw [ evalAt ];
     unfold BranchingProgram.evalAt;
     rw [ WellFounded.fix_eq ];
     unfold toBranchingProgram; aesop;
-  · unfold BranchingProgram.evalAt evalFrom
+  · unfold BranchingProgram.evalAt evalAt
     convert ih (L.edges u (x (L.nodeVar u))) using 1
     · rw [BranchingProgram.evalAt, WellFounded.fix_eq]
       simp [toBranchingProgram, Fin.lastCases]
@@ -302,7 +473,184 @@ The DAG conversion `LayeredBranchingProgram.toBranchingProgram` preserves semant
 @[simp]
 theorem toBranchingProgram_eval : L.toBranchingProgram.eval = L.eval := by
   funext x
-  convert ← toBranchingProgram_evalAt_eq_evalFrom L x 0 L.start
-  exact evalFrom_evalLayer_eq_eval L x 0
+  convert ← toBranchingProgram_evalAt_eq_evalAt L x 0 L.start
+  exact evalAt_evalLayer_eq_eval L x 0
 
 end LayeredBranchingProgram
+
+namespace BranchingProgram
+
+variable {α : Type u} {β : Type v} {γ : Type w} (P : BranchingProgram α β γ) [Fintype P.nodes]
+
+/--
+Conversion from `BranchingProgram` to `SkipBranchingProgram`.
+Restricts nodes to those reachable from the start node.
+-/
+def toSkipBranchingProgram : SkipBranchingProgram α β γ where
+  depth := P.depth
+  nodes := fun i ↦ { u : P.nodes // P.height u = P.depth - i ∧ P.Reachable u }
+  nodeVar := fun {i} ⟨u, hu⟩ ↦
+    match h : P.info u with
+    | .inl _ => Classical.choice (by
+    -- Since there's a path from u to v, there must be at least one variable in α that's involved in the edges of the path.
+    have h_var : ∃ var : α, ∃ next : β → P.nodes, P.info u = Sum.inr (var, next) := by
+      have h_var : 0 < P.height u := by
+        rw [ hu.1 ];
+        exact Nat.sub_pos_of_lt ( Fin.is_lt i );
+      exact is_internal_of_height_pos P u h_var;
+    exact ⟨ h_var.choose ⟩)
+    | .inr (var, _) => var
+  edges := fun {i} ⟨u, hu⟩ b ↦
+    match h : P.info u with
+    | .inl _ => Classical.choice (by
+    exact ⟨ ⟨ i.castSucc, u, hu ⟩ ⟩)
+    | .inr (var, next) =>
+        let v := next b
+        let hv := P.height v
+        let j := P.depth - hv
+        ⟨⟨j, by
+          exact Nat.lt_succ_of_le ( Nat.sub_le _ _ )⟩, ⟨v, by
+          -- Since $v$ is reachable from $u$ and $u$ is reachable from the start, $v$ is reachable from the start.
+          have hv_reachable : P.Reachable v := by
+            exact hu.2.tail ( by exact ⟨ var, next, h, b, rfl ⟩ );
+          exact ⟨ by rw [ Nat.sub_sub_self ( show hv ≤ P.depth from P.height_le_of_reachable hv_reachable ) ], hv_reachable ⟩⟩⟩
+  edges_layer_gt := fun {i} ⟨u, hu⟩ b ↦ by
+    by_cases h : ∃ var next, P.info u = .inr (var, next);
+    · rcases h with ⟨ var, next, h ⟩;
+      convert Nat.lt_sub_of_add_lt _;
+      rotate_left;
+      exact P.height ( next b );
+      exact 0;
+      exact P.depth - i.castSucc;
+      · exact lt_of_lt_of_le ( BranchingProgram.height_child_lt _ _ _ _ h _ ) ( by omega );
+      · grind;
+    · cases h' : P.info u <;> simp_all +decide;
+      · have := hu.1 ▸ BranchingProgram.height_eq_zero_of_leaf P u _ h'; simp_all +decide ;
+        exact absurd this ( Nat.sub_ne_zero_of_lt ( Fin.is_lt i ) );
+      · exact False.elim <| h _ _ rfl
+  startUnique := {
+    default := ⟨P.start, by simp [depth, Reachable]; rfl⟩
+    uniq := fun ⟨u, hu⟩ ↦ by
+      exact Subtype.ext <| eq_start_of_reachable_and_height_eq P hu.2 <| by simpa using hu.1;
+  }
+  retVals := fun ⟨u, hu⟩ ↦
+    match h : P.info u with
+    | .inl res => res
+    | .inr _ => Classical.choice (by
+    -- Since the branching program must return a value in γ when it reaches a leaf node, γ cannot be empty.
+    have h_nonempty : ∃ x : P.nodes, ∃ res : γ, P.info x = .inl res := by
+      have h_nonempty : ∃ x : P.nodes, P.height x = 0 := by
+        exact ⟨ u, hu.1.trans ( Nat.sub_self _ ) ⟩;
+      exact h_nonempty.elim fun x hx => by obtain ⟨ res, hres ⟩ := BranchingProgram.is_leaf_of_height_zero P x hx; exact ⟨ x, res, hres ⟩ ;
+    exact ⟨ h_nonempty.choose_spec.choose ⟩)
+
+@[simp]
+theorem toSkipBranchingProgram_depth :
+    P.toSkipBranchingProgram.depth = P.depth :=
+  rfl
+
+@[simp]
+theorem toSkipBranchingProgram_start :
+    P.toSkipBranchingProgram.start.val = P.start :=
+  rfl
+
+theorem toSkipBranchingProgram_evalAt
+    (x : α → β) (i : Fin P.depth.succ) (u : P.toSkipBranchingProgram.nodes i) :
+    P.toSkipBranchingProgram.evalAt x u = P.evalAt x u.1 := by
+  induction' n : P.toSkipBranchingProgram.depth - i.val using Nat.strong_induction_on with n ih generalizing i u;
+  unfold SkipBranchingProgram.evalAt
+  split_ifs with h;
+  · unfold BranchingProgram.evalAt;
+    have h_layer : P.height u.val = P.depth - i := by
+      exact u.2.1;
+    have h_leaf : ∃ res, P.info u.val = .inl res := by
+      convert leaf_of_layer_eq_depth P u.val _;
+      rw [ h_layer, h, Fin.val_last, toSkipBranchingProgram_depth ];
+    rw [ WellFounded.fix_eq ];
+    unfold BranchingProgram.toSkipBranchingProgram; aesop;
+  · convert ih _ _ _ _ rfl using 1;
+    · unfold BranchingProgram.evalAt;
+      rw [ WellFounded.fix_eq, WellFounded.fix_eq ];
+      unfold BranchingProgram.toSkipBranchingProgram
+      simp
+      let h_info := P.info u.val
+      cases h : h_info
+      · exact absurd ( u.2.1 ) ( by
+          have := BranchingProgram.height_eq_zero_of_leaf P u.val _ h;
+          exact ne_of_lt ( lt_of_le_of_lt ( Nat.le_of_eq this ) ( Nat.sub_pos_of_lt ( lt_of_le_of_ne ( Fin.le_last _ ) ( by simpa [ Fin.ext_iff ] using ‹¬i = Fin.last _› ) ) ) ) );
+      · subst h_info
+        sorry
+    · rw [ ← n ];
+      apply Nat.sub_lt_sub_left
+      · exact lt_of_le_of_ne ( Fin.le_last _ ) ( by simpa [ Fin.ext_iff ] using h );
+      · convert P.toSkipBranchingProgram.edges_layer_gt _ _;
+        rotate_left;
+        exact Fin.castPred i h;
+        exact ⟨ u.1, by simpa [ Fin.castSucc_castPred ] using u.2 ⟩;
+        exact x ( P.toSkipBranchingProgram.nodeVar ( Fin.castSucc_castPred i h ▸ u ) );
+        exact Fin.val_fin_lt
+
+/--
+The conversion from BranchingProgram to SkipBranchingProgram preserves semantics (eval).
+-/
+@[simp]
+theorem toSkipBranchingProgram_eval : P.toSkipBranchingProgram.eval = P.eval := by
+  ext1
+  rw [SkipBranchingProgram.eval, eval, toSkipBranchingProgram_evalAt, toSkipBranchingProgram_start]
+
+end BranchingProgram
+
+namespace SkipBranchingProgram
+open Classical
+
+variable {α : Type u} {β : Type v} {γ : Type w} (P : SkipBranchingProgram α β γ)
+
+/--
+If a SkipBranchingProgram has depth > 0, then α must be nonempty because the start node
+at layer 0 must read a variable.
+-/
+theorem nonempty_of_depth_pos (h : 0 < P.depth) : Nonempty α :=
+  let z : Fin P.depth := ⟨0, h⟩
+  let u : P.nodes z.castSucc := cast (by simp [z]) P.start
+  ⟨P.nodeVar u⟩
+
+/--
+Conversion from `SkipBranchingProgram` to `LayeredBranchingProgram`.
+Adds dummy nodes to carry values across skipped layers.
+-/
+def toLayeredBranchingProgram : LayeredBranchingProgram α β γ where
+  depth := P.depth
+  nodes i := (P.nodes i) ⊕ Σ (j : Fin P.depth.succ), { v : P.nodes j // j > i ∧ i.val > 0 }
+  nodeVar {i} u := match u with
+    | .inl u => P.nodeVar u
+    | .inr _ =>
+      if h : Nonempty (P.nodes i.castSucc) then
+        P.nodeVar (Classical.choice h)
+      else
+        (P.nonempty_of_depth_pos (by linarith [i.2])).some
+  edges {i} u b := match u with
+    | .inl u =>
+      let next := P.edges u b
+      let m := next.1
+      let v := next.2
+      if h : m = i.succ then
+        .inl (h ▸ v)
+      else
+        .inr ⟨m, ⟨v, ⟨lt_of_le_of_ne (P.edges_layer_gt u b) (Ne.symm h), i.succ_pos⟩⟩⟩
+    | .inr ⟨m, ⟨v, ⟨hm, _⟩⟩⟩ =>
+      if h : m = i.succ then
+        .inl (h ▸ v)
+      else
+        .inr ⟨m, ⟨v, ⟨lt_of_le_of_ne (Nat.succ_le_of_lt hm) (Ne.symm h), i.succ_pos⟩⟩⟩
+  startUnique := {
+    default := .inl P.start
+    uniq u := by
+      cases u
+      · simpa using P.startUnique.uniq _
+      · aesop
+  }
+  retVals u := match u with
+    | .inl u => P.retVals u
+    | .inr ⟨_, ⟨_, ⟨h, _⟩⟩⟩ => (h.not_ge (Fin.le_last _)).elim
+
+end SkipBranchingProgram
